src/CoreData/CoreData.v
@@ -1,2 +1,3 @@
 Require Export ZXCore.
 Require Export Proportional.
+Require Export Swaps.
