src/CoreData/Swaps.v
@@ -1,0 +1,56 @@
+Require Import ZXCore.
+Require Export QuantumLib.Quantum.
+
+Open Scope ZX_scope.
+
+Fixpoint top_to_bottom_helper (n : nat) : ZX (S n) (S n) :=
+  match n with 
+  | 0   => Wire
+  | S k => Compose (Stack Swap (n_wire k)) (Stack Wire (top_to_bottom_helper k))
+  end.
+
+Definition top_to_bottom (n : nat) : ZX n n :=
+  match n with
+  | 0 => Empty
+  | S k => top_to_bottom_helper k
+  end.
+
+Definition bottom_to_top (n : nat) : ZX n n :=
+  (top_to_bottom n)⊤.
+
+Definition a_swap (n : nat) : ZX n n :=
+  match n with
+  | 0   => Empty
+  | S k => bottom_to_top (S k) ⟷ (— ↕ top_to_bottom k)
+  end.
+
+(* Arbitrary Swap Semantics *)
+
+(* A linear mapping which takes | x y1 ... yn > -> | y1 .. yn x > *)
+Fixpoint top_wire_to_bottom (n : nat) : Square (2 ^ n) :=
+  match n with
+  | 0   => I 1
+  | S k => match k with
+           | 0   => I 2
+           | S j => (@Mmult _ (2^n) _) ((I 2) ⊗ (top_wire_to_bottom k)) (swap ⊗ (j ⨂ (I 2)))
+           end
+  end.
+
+Open Scope matrix_scope.
+Definition bottom_wire_to_top (n : nat) : Square (2 ^ n) :=
+  (top_wire_to_bottom n)⊤.
+
+Definition a_swap_semantics (n : nat) : Square (2 ^ n) :=
+  match n with
+  | 0   => I 1
+  | S k => (@Mmult _ (2 ^ n) _ ((I 2) ⊗ top_wire_to_bottom (k)) ((bottom_wire_to_top (S k))))
+  end.
+
+Fixpoint n_swap (n : nat) : ZX n n :=
+  match n with 
+  | 0 => ⦰ 
+  | 1 => —
+  | (S (S n)) => a_swap (S (S n)) ⟷ (— ↕ (@cast _ _ (n + 1)%nat (n + 1)%nat (eq_sym (@Nat.add_1_r n)) (eq_sym (@Nat.add_1_r n)) (n_swap n ↕ —)))
+  end.
+  
+  
